VRF Prove

VRF/Hacl.VRF.Hash.fst
@@ -4,121 +4,120 @@ open FStar.Mul
 
 open FStar.HyperStack
 open FStar.HyperStack.ST
+module ST = FStar.HyperStack.ST
 
 open Spec.Lib
 open Spec.Lib.IntSeq
 
 open Spec.Lib.IntTypes
 open Spec.Lib.IntBuf
-
-open Spec.Lib.IntSeq.Lemmas
 open Spec.Lib.IntBuf.Lemmas
 
-open Hacl.VRF.HashToCurve
+open Hacl.VRF.HashToCurveFinal
 open Hacl.VRF.HashPoints
-open Hacl.VRF.Bignum
+(* open Hacl.VRF.Bignum *)
 
 open Hacl.VRF.Lib
 
-(*
-let g_x : elem = 15112221349535400772501151409588531511454012693041857206046113283949847762202
-let g_y : elem = 46316835694926478169428394003475163141307993866256225615783033603165251855960
-*)
-
-(*
-corresponds to edd25519 method make_g
-*)
+#reset-options " --z3rlimit 100"
 
 
 (* Secret buffer consists of private key of the user and the random value *)
 (* Input - the array to be hashed *)
 (* pk - public key of the user *)
 
+val _ECVRF_prove_2: proof: lbuffer uint8 80 -> secret: doubleWord -> Stack bool
+	(requires(fun h0 -> live h0 proof /\ live h0 secret /\ disjoint proof secret))
+	(ensures (fun h0 _ h1 -> preserves_live h0 h1 /\ modifies1 proof h0 h1))
+
+let _ECVRF_prove_2 proof secret = 
+	alloc #_ #(bool) #(30) (size 30) (u64(0))
+		[BufItem secret; BufItem proof] [BufItem proof]
+		(fun h0 _ h1 -> True)
+		(fun bigNums -> 
+			let cf = sub #_ #(30) #(5) bigNums (size 0) (size 5) in 
+			let xf = sub #_ #(30) #(5) bigNums (size 5) (size 5) in 
+			let cxf = sub #_ #(30) #(5) bigNums (size 10) (size 5) in 
+			let kf = sub #_ #(30) #(5) bigNums (size 15) (size 5) in 
+
+			let c = sub #_ #(80) #(32) proof (size 32) (size 32) in 
+			let s = sub #_ #(80) #(32) proof (size 48) (size 32) in 
+
+			let clow = sub #_ #(80) #(16) proof (size 48) (size 16) in 
+			let chigh = sub #_ #(80) #(16) proof (size 32) (size 16) in 
+
+			let privateKey = sub #_ #(64) #(32) secret (size 0) (size 32) in 
+			let random = sub #_ #(64) #(32) secret (size 32) (size 32) in 
+				
+			fexpand cf c;
+				disjoint_sub_lemma2 bigNums (size 0) (size 5) (size 5) (size 5);
+				disjoint_sub_lemma2 bigNums (size 0) (size 5) (size 15) (size 5);
+				disjoint_sub_lemma2 bigNums (size 5) (size 5) (size 15) (size 5);
+				disjoint_sub_lemma2 bigNums (size 10) (size 5) (size 15) (size 5);
+			fexpand xf privateKey;
+			fexpand kf random; 
+				let h0 = ST.get() in 
+				lemma_red_513_is_red_53 (as_lseq cf h0);
+				lemma_red_513_is_red_5413 (as_lseq xf h0);
+			fmul cxf cf xf; 
+				let h3 = ST.get() in 
+				disjoint_sub_lemma2 bigNums (size 15) (size 5) (size 10) (size 5);
+			fdifference_reduced kf cxf; 
+			fcontract s kf;
+			copy (size 16) chigh clow;	
+			true
+		)
+
+
 val _ECVRF_prove: 
 	#len : size_nat -> 
 	proof: lbuffer uint8 80 -> 
-	inputLength: size_t{v inputLength == len } -> 
+	inputLength: size_t{v inputLength == len /\ len < maxint SIZE - 96} -> 
 	input: lbuffer uint8 len -> 
 	secret: doubleWord ->
 	pk: point  -> 
 	Stack bool 
-		(requires 
-			(fun h0 -> live h0 proof /\ live h0 input /\ live h0 secret /\ live h0 pk 
-			)
-		)
-		(ensures 
-			(
-				fun h0 _ h1 -> preserves_live h0 h1
-			) 
-		)
+		(requires (fun h0 -> live h0 proof /\ live h0 input /\ live h0 secret /\ live h0 pk /\ disjoint proof secret))
+		(ensures (fun h0 _ h1 -> preserves_live h0 h1))
 
 let _ECVRF_prove #len proof inputLength input secret pk = 
-	let r = alloc #_ #(bool) (size 120) (u128(0)) 
+	let r = alloc #_ #(bool) (size 120) (u64(0)) 
 		[BufItem input; BufItem secret; BufItem pk] [BufItem proof] 
 		(fun h0 _ h1 -> True) 
 		(fun pointBuffer ->
-
 			let c = sub proof (size 32) (size 32) in 
 
 			let privateKey = sub #_ #(64) #(32) secret (size 0) (size 32) in 
 			let random = sub #_ #(64) #(32) secret (size 32) (size 32) in 
 
 			let generator = sub pointBuffer (size 0) (size 20) in 
-				generatorLoad generator;
+			make_g generator;
 			let h = sub #_ #(120) #(20) pointBuffer (size 20) (size 20) in
-				let r = _ECVRF_hash_to_curve h pk inputLength input in 
-				if not r then false else 
-			(let publicKey =  sub #_ #(120) #(20) pointBuffer (size 40) (size 20) in
-				copy (size 20) publicKey pk;
-			let gammaPoint = sub #_ #(120) #(20) pointBuffer (size 60) (size 20) in
-				point_mult gammaPoint h privateKey;
-			let gk = sub #_ #(120) #(20) pointBuffer (size 80) (size 20) in
-				point_mult gk generator random;
-			let hk = sub #_ #(120) #(20) pointBuffer (size 100) (size 20) in
-				point_mult hk h random;
-			 _ECVRF_hashPoints c pointBuffer;
-			true)
+				disjoint_sub_lemma1 pointBuffer pk (size 20) (size 20);
+			let r = _ECVRF_hash_to_curve h pk inputLength input in 
+			if not r then begin
+				false
+			end
+			else begin
 
+				let publicKey =  sub #_ #(120) #(20) pointBuffer (size 40) (size 20) in
+				copy (size 20) pk publicKey;
+				let gammaPoint = sub #_ #(120) #(20) pointBuffer (size 60) (size 20) in
+					point_mult gammaPoint h privateKey;
+				let gk = sub #_ #(120) #(20) pointBuffer (size 80) (size 20) in
+					point_mult gk generator random;
+				let hk = sub #_ #(120) #(20) pointBuffer (size 100) (size 20) in
+					point_mult hk h random;
+
+				disjoint_sub_lemma1 proof pointBuffer (size 32) (size 32);	
+
+				 _ECVRF_hashPoints c pointBuffer;
+				true
+			end
 		) 
 	in 
-		(
-			if  not r then false else  
-				(
-					alloc #_ #(bool) #(30) (size 30) (u64(0))
-					[BufItem secret; BufItem proof] [BufItem proof]
-					(fun h0 _ h1 -> True)
-					(fun bigNums -> 
-
-					let cf = sub #_ #(30) #(5) bigNums (size 0) (size 5) in 
-					let xf = sub #_ #(30) #(5) bigNums (size 5) (size 5) in 
-					let cxf = sub #_ #(30) #(5) bigNums (size 10) (size 5) in 
-					let kf = sub #_ #(30) #(5) bigNums (size 15) (size 5) in 
-					(*let k_cxf = sub #_ #(30) #(5) bigNums (size 20) (size 5) in 
-					let resultf = sub #_ #(30) #(5) bigNums (size 25) (size 5) in *)
-
-					let c = sub #_ #(80) #(32) proof (size 32) (size 32) in 
-					let s = sub #_ #(80) #(32) proof (size 48) (size 32) in 
-
-					let privateKey = sub #_ #(64) #(32) secret (size 0) (size 32) in 
-					let random = sub #_ #(64) #(32) secret (size 32) (size 32) in 
-
-					fexpand cf c; 
-					fexpand xf privateKey;
-					fexpand kf random; (* kf = random *)
-
-					fmul cxf cf xf; (*cxf = c * x *)
-					fdifference_reduced kf cxf; (* kf = kf - cxf *)
-
-					let clow = sub #_ #(80) #(16) proof (size 48) (size 16) in 
-					let chigh = sub #_ #(80) #(16) proof (size 32) (size 16) in 
-					copy (size 16) clow chigh;
-
-					fcontract s kf;
- 
-					true
-					)
-				)
-			)
+		if  not r then false else  
+			_ECVRF_prove_2 proof secret
 
 (*)
 val decodeProof: gamma: point -> 
